Weidenbach_Book/IsaSAT_VMTF.thy
@@ -120,10 +120,10 @@ end
 
 
 definition (in -) insert_sort_inner_nth :: \<open>nat_vmtf_node list \<Rightarrow> nat list \<Rightarrow> nat \<Rightarrow> nat list nres\<close> where
-  \<open>insert_sort_inner_nth ns = insert_sort_inner (\<lambda>remove n. stamp (ns ! (remove ! n)))\<close>
+  \<open>insert_sort_inner_nth ns = insert_sort_inner (<) (\<lambda>remove n. stamp (ns ! (remove ! n)))\<close>
 
 definition (in -) insert_sort_nth :: \<open>nat_vmtf_node list \<times> 'c \<Rightarrow> nat list \<Rightarrow> nat list nres\<close> where
-  \<open>insert_sort_nth = (\<lambda>(ns, _). insert_sort (\<lambda>remove n. stamp (ns ! (remove ! n))))\<close>
+  \<open>insert_sort_nth = (\<lambda>(ns, _). insert_sort (<) (\<lambda>remove n. stamp (ns ! (remove ! n))))\<close>
 
 
 lemma (in -) insert_sort_inner_nth_code_helper:
